VST-introduction/VSU_kalloc_kfree_definitions.v
@@ -8,9 +8,6 @@ Require Import malloc_sep.*)
 (* THIS SHOULD CONTAIN ANY INTERNAL FUNCTIONS... I DON'T HAVE ANY *)
 
 
-(** token -- could be moved to another file *)
-(*** kalloc token size... *)
-(***** kalloc token size ******)
 Definition kalloc_token_sz (sh: share) (n: Z) (p: val) : mpred :=
   !! ((*field_compatible t_run [] p /\*)
       0 < n <= PGSIZE
@@ -35,54 +32,7 @@ Proof.
   intros. 
   unfold kalloc_token_sz. simpl. entailer.
 Qed.
-
-(******************************)
-
-(*** kalloc token type... *)
-Definition my_kalloc_token {cs: compspecs} sh t p :=
-  !! field_compatible t [] p && (* this shoudl work because of memory_block_data_at_*)
-  (kalloc_token_sz sh (sizeof t) p).
-
-Lemma my_kalloc_token_valid_pointer:
-  forall (sh : share) (t : type) (p : val),
-  my_kalloc_token sh t p |-- valid_pointer p.
-Proof.
-  intros. 
-  unfold my_kalloc_token. unfold kalloc_token_sz. entailer!.
-Qed.
-
-Ltac kalloc_token_data_at_valid_pointer :=
-  match goal with |- ?A |-- valid_pointer ?p =>
-   match A with
-   | context [my_kalloc_token _ _ ?t p] =>
-         try (assert (sizeof t <= 0)
-	  by (simpl sizeof in *; rep_lia); fail 1);
-         try (assert (sizeof t > 0)
-	  by (simpl sizeof in *; rep_lia); fail 1);
-         destruct (zlt 0 (sizeof t));
-         auto with valid_pointer
-   | context [kalloc_token_sz _ _ ?n p] =>
-         try (assert (n <= 0) by rep_lia; fail 1);
-         try (assert (n > 0) by rep_lia; fail 1);
-         destruct (zlt 0 n);
-         auto with valid_pointer
-   end
- end.
-
-#[export] Hint Extern 1 (my_kalloc_token _ _ _ _ |-- valid_pointer _) =>
-  (simple apply my_kalloc_token_valid_pointer; data_at_valid_aux) : valid_pointer.
-#[export] Hint Extern 4 (_ |-- valid_pointer _) => kalloc_token_data_at_valid_pointer : valid_pointer.
-
-Lemma my_kalloc_token_local_facts:  forall {cs: compspecs} sh t p,
-      my_kalloc_token sh t p |-- !! (field_compatible t [] p /\ malloc_compatible (sizeof t) p).
-Proof. intros.
- unfold my_kalloc_token.
- normalize. rewrite prop_and.
- apply andp_right. apply prop_right; auto.
- apply kalloc_token_sz_local_facts.
-Qed.
-#[export] Hint Resolve my_kalloc_token_local_facts : saturate_local.
-
+(***** kalloc token size ******)
 
 
 Definition Tok_APD := Build_KallocTokenAPD kalloc_token_sz kalloc_token_sz_valid_pointer
@@ -130,18 +80,6 @@ Proof.
   intros. apply pred_ext.
   - unfold kalloc_token_sz. entailer.
   - unfold kalloc_token_sz. entailer!.
-Qed.
-
-Lemma my_kalloc_token_split: 
- forall (sh: share) (t: type) (p: val),
- my_kalloc_token (sh) (t) (p)
-  = 
-  !! field_compatible t [] p &&
-  (kalloc_token_sz sh (sizeof t) p).
-Proof.
-  intros. apply pred_ext.
-  - unfold my_kalloc_token. entailer.
-  - unfold my_kalloc_token. entailer!.
 Qed.
 
 (************ lemmas etc. end *************)
